Typing, conversion and evaluation

theories/Typing.v
@@ -2,6 +2,7 @@ Require Import List Program.
 Require Import Template.Template Template.Ast.
 Require Import BinPos.
 Require Import Coq.Arith.Compare_dec.
+Set Asymmetric Patterns.
 
 Definition on_snd {A B} (f : B -> B) (p : A * B) :=
   let '(x, y) := p in (x, f y).
@@ -30,7 +31,7 @@ Fixpoint lift n k t : term :=
   | tCoFix mfix k =>
     let k' := List.length mfix + k in
     let mfix' := List.map (map_def (lift n k')) mfix in
-    tCoFix mfix k
+    tCoFix mfix' k
   | x => x
   end.
 
@@ -48,8 +49,8 @@ Fixpoint subst t k u :=
   | tLambda na T M => tLambda na (subst t k T) (subst t (S k) M)
   | tApp u v => tApp (subst t k u) (List.map (subst t k) v)
   | tProd na A B => tProd na (subst t k A) (subst t (S k) B)
-  | tCast c kind t => tCast (subst t k c) kind (subst t k t)
-  | tLetIn na b t b' => tLetIn na (subst t k b) (subst t k t) (subst t (S k) b')
+  | tCast c kind ty => tCast (subst t k c) kind (subst t k ty)
+  | tLetIn na b ty b' => tLetIn na (subst t k b) (subst t k ty) (subst t (S k) b')
   | tCase ind p c brs =>
     let brs' := List.map (on_snd (subst t k)) brs in
     tCase ind (subst t k p) (subst t k c) brs'
@@ -61,7 +62,7 @@ Fixpoint subst t k u :=
   | tCoFix mfix k =>
     let k' := List.length mfix + k in
     let mfix' := List.map (map_def (subst t k')) mfix in
-    tCoFix mfix k
+    tCoFix mfix' k
   | x => x
   end.
 
@@ -371,11 +372,6 @@ Next Obligation.
   split; auto.
 Qed.
   
-Reserved Notation " Σ ; Γ |-- t : T " (at level 70, t, T at next level). 
-Reserved Notation " Σ ; Γ |-- t = u " (at level 70, t, u at next level). 
-
-Notation " Γ ,, d " := (snoc Γ d) (at level 20, d at next level).
-
 Definition max_sort (s1 s2 : sort) : sort := s2. (* FIXME *)
 
 Fixpoint mktApp t l :=
@@ -409,8 +405,16 @@ Definition is_constructor n ts :=
   | None => false
   end.
 
-Definition iota_red c args brs :=
-  (mktApp (snd (List.nth c brs (0, tRel 0))) args).  
+Definition tAppnil t l :=
+  match l with
+  | nil => t
+  | _ => tApp t l
+  end.
+
+Definition iota_red npar c args brs :=
+  (mktApp (snd (List.nth c brs (0, tRel 0))) (List.skipn npar args)).
+
+Notation " Γ ,, d " := (snoc Γ d) (at level 20, d at next level).
 
 Inductive red1 (Σ : global_context) (Γ : context) : term -> term -> Prop :=
 (** Reductions *)
@@ -424,12 +428,12 @@ Inductive red1 (Σ : global_context) (Γ : context) : term -> term -> Prop :=
 
 | red_rel i (isdecl : i < List.length Γ) body :
     (safe_nth Γ (exist _ i isdecl)).(decl_body) = Some body ->
-    red1 Σ Γ (tRel i) (lift0 i body) 
+    red1 Σ Γ (tRel i) (lift0 (S i) body) 
          
 (** Case *)
 | red_iota ind pars c args p brs :
     red1 Σ Γ (tCase (ind, pars) p (mktApp (tConstruct ind c) args) brs)
-         (iota_red c args brs)
+         (iota_red pars c args brs)
 
 (** Fix unfolding, with guard *)
 | red_fix mfix idx args narg fn :
@@ -478,6 +482,7 @@ Inductive red Σ Γ M : term -> Prop :=
 | refl_red : red Σ Γ M M
 | trans_red : forall (P : term) N, red Σ Γ M P -> red1 Σ Γ P N -> red Σ Γ M N.
 
+
 Section Forallb2.
   Context {A} (f : A -> A -> bool).
 
@@ -497,8 +502,29 @@ Definition eq_sort s s' :=
   | _, _ => false
   end.
 
+Definition leq_sort s s' :=
+  match s, s' with
+  | sProp, _ => true
+  | sSet, sSet => true
+  | sSet, sType _ => true
+  | sType p, sType q => true (* Pos.leb p q  *)(* FIXME incorrect *)
+  | _, _ => false
+  end.
+
 Definition eq_string s s' :=
   if string_dec s s' then true else false.
+
+Definition eq_ind i i' :=
+  let 'mkInd i n := i in
+  let 'mkInd i' n' := i' in
+  eq_string i i' && Nat.eqb n n'.
+
+Definition eq_constant := eq_string.
+
+Arguments dname {term} _.
+Arguments dtype {term} _.
+Arguments dbody {term} _.
+Arguments rarg {term} _.
 
 Fixpoint eq_term (t u : term) {struct t} :=
   match t, u with
@@ -509,94 +535,155 @@ Fixpoint eq_term (t u : term) {struct t} :=
   | tSort s, tSort s' => eq_sort s s'
   | tApp f args, tApp f' args' => eq_term f f' && forallb2 eq_term args args'
   | tCast t _ v, tCast u _ v' => eq_term t u && eq_term v v'
-  | tConst c, tConst c' => eq_string c c'
-  | tInd (mkInd i n), tInd (mkInd i' n') => eq_string i i' && Nat.eqb n n'
-  | tConstruct (mkInd i n) k, tConstruct (mkInd i' n') k' =>
-    eq_string i i' && Nat.eqb n n' && Nat.eqb k k'
+  | tConst c, tConst c' => eq_constant c c'
+  | tInd i, tInd i' => eq_ind i i'
+  | tConstruct i k, tConstruct i' k' => eq_ind i i' && Nat.eqb k k'
   | tLambda _ b t, tLambda _ b' t' => eq_term b b' && eq_term t t'
   | tProd _ b t, tProd _ b' t' => eq_term b b' && eq_term t t'
+  | tCase (ind, par) p c brs,
+    tCase (ind',par') p' c' brs' =>
+    eq_term p p' && eq_term c c' && forallb2 (fun '(a, b) '(a', b') => eq_term b b') brs brs'
+  | tProj p c, tProj p' c' => eq_constant p p' && eq_term c c'
+  | tFix mfix idx, tFix mfix' idx' =>
+    forallb2 (fun x y =>
+                eq_term x.(dtype) y.(dtype) && eq_term x.(dbody) y.(dbody)) mfix mfix' &&
+    Nat.eqb idx idx'
+  | tCoFix mfix idx, tCoFix mfix' idx' =>
+    forallb2 (fun x y =>
+                eq_term x.(dtype) y.(dtype) && eq_term x.(dbody) y.(dbody)) mfix mfix' &&
+    Nat.eqb idx idx'
+  | _, _ => false
+  end.
+
+Fixpoint leq_term (t u : term) {struct t} :=
+  match t, u with
+  | tRel n, tRel n' => Nat.eqb n n'
+  | tMeta n, tMeta n' => Nat.eqb n n'
+  | tEvar ev args, tEvar ev' args' => Nat.eqb ev ev' && forallb2 eq_term args args'
+  | tVar id, tVar id' => eq_string id id'
+  | tSort s, tSort s' => leq_sort s s'
+  | tApp f args, tApp f' args' => eq_term f f' && forallb2 eq_term args args'
+  | tCast t _ v, tCast u _ v' => leq_term t u
+  | tConst c, tConst c' => eq_constant c c'
+  | tInd i, tInd i' => eq_ind i i'
+  | tConstruct i k, tConstruct i' k' => eq_ind i i' && Nat.eqb k k'
+  | tLambda _ b t, tLambda _ b' t' => eq_term b b' && eq_term t t'
+  | tProd _ b t, tProd _ b' t' => eq_term b b' && leq_term t t'
+  | tCase (ind, par) p c brs,
+    tCase (ind',par') p' c' brs' =>
+    eq_term p p' && eq_term c c' && forallb2 (fun '(a, b) '(a', b') => eq_term b b') brs brs'
+  | tProj p c, tProj p' c' => eq_constant p p' && eq_term c c'
+  | tFix mfix idx, tFix mfix' idx' =>
+    forallb2 (fun x y =>
+                eq_term x.(dtype) y.(dtype) && eq_term x.(dbody) y.(dbody)) mfix mfix' &&
+    Nat.eqb idx idx'
+  | tCoFix mfix idx, tCoFix mfix' idx' =>
+    forallb2 (fun x y =>
+                eq_term x.(dtype) y.(dtype) && eq_term x.(dbody) y.(dbody)) mfix mfix' &&
+    Nat.eqb idx idx'
   | _, _ => false (* Case, Proj, Fix, CoFix *)
   end.
 
+Reserved Notation " Σ ;;; Γ |-- t : T " (at level 50, Γ, t, T at next level).
+Reserved Notation " Σ ;;; Γ |-- t <= u " (at level 50, Γ, t, u at next level). 
+
 Inductive typing (Σ : global_context) (Γ : context) : term -> term -> Prop :=
 | type_Rel n : forall (isdecl : n < List.length Γ),
-    Σ ; Γ |-- (tRel n) : lift0 n (safe_nth Γ (exist _ n isdecl)).(decl_type)
+    Σ ;;; Γ |-- (tRel n) : lift0 (S n) (safe_nth Γ (exist _ n isdecl)).(decl_type)
 
 | type_Sort s :
-    Σ ; Γ |-- (tSort s) : tSort (succ_sort s)
+    Σ ;;; Γ |-- (tSort s) : tSort (succ_sort s)
 
-| type_Cast c k t :
-    Σ ; Γ |-- (tCast c k t) : t 
+| type_Cast c k t s :
+    Σ ;;; Γ |-- t : tSort s ->
+    Σ ;;; Γ |-- c : t ->
+    Σ ;;; Γ |-- (tCast c k t) : t 
 
 | type_Prod n t b s1 s2 :
-    Σ ; Γ |-- t : tSort s1 ->
-    Σ ; Γ ,, vass n t |-- b : tSort s2 ->
-    Σ ; Γ |-- (tProd n t b) : tSort (max_sort s1 s2)
+    Σ ;;; Γ |-- t : tSort s1 ->
+    Σ ;;; Γ ,, vass n t |-- b : tSort s2 ->
+    Σ ;;; Γ |-- (tProd n t b) : tSort (max_sort s1 s2)
 
-| type_Lambda n t b bty :
-    Σ ; Γ ,, vass n t |-- b : bty ->
-    Σ ; Γ |-- (tLambda n t b) : tProd n t bty
+| type_Lambda n t b s1 bty :
+    Σ ;;; Γ |-- t : tSort s1 ->
+    Σ ;;; Γ ,, vass n t |-- b : bty ->
+    Σ ;;; Γ |-- (tLambda n t b) : tProd n t bty
 
-| type_LetIn n b b_ty b' b'_ty :
-    Σ ; Γ ,, vdef n b b_ty |-- b' : b_ty ->
-    Σ ; Γ |-- (tLetIn n b b_ty b') : tLetIn n b b_ty b'_ty
+| type_LetIn n b b_ty b' s1 b'_ty :
+    Σ ;;; Γ |-- b_ty : tSort s1 ->
+    Σ ;;; Γ |-- b : b_ty -> 
+    Σ ;;; Γ ,, vdef n b b_ty |-- b' : b'_ty ->
+    Σ ;;; Γ |-- (tLetIn n b b_ty b') : tLetIn n b b_ty b'_ty
 
 | type_App t l t_ty t' :
-    Σ ; Γ |-- t : t_ty ->
+    Σ ;;; Γ |-- t : t_ty ->
     typing_spine Σ Γ t_ty l t' ->
-    Σ ; Γ |-- (tApp t l) : t'          
+    Σ ;;; Γ |-- (tApp t l) : t'          
 
 | type_Const cst :
     forall (isdecl : declared_constant Σ cst),
-    Σ ; Γ |-- (tConst cst) : type_of_constant Σ (exist _ cst isdecl)
+    Σ ;;; Γ |-- (tConst cst) : type_of_constant Σ (exist _ cst isdecl)
 
 | type_Ind ind :
     forall (isdecl : declared_inductive Σ ind),
-    Σ ; Γ |-- (tInd ind) : type_of_inductive Σ (exist _ ind isdecl)
+    Σ ;;; Γ |-- (tInd ind) : type_of_inductive Σ (exist _ ind isdecl)
 
 | type_Construct ind i :
     forall (isdecl : declared_constructor Σ (ind, i)),
-    Σ ; Γ |-- (tConstruct ind i) : type_of_constructor Σ (exist _ (ind,i) isdecl)
+    Σ ;;; Γ |-- (tConstruct ind i) : type_of_constructor Σ (exist _ (ind,i) isdecl)
 
 | type_Case indpar p c brs args :
-    Σ ; Γ |-- c : mktApp (tInd (fst indpar)) args ->
+    Σ ;;; Γ |-- c : mktApp (tInd (fst indpar)) args ->
     (** TODO check brs *)                  
-    Σ ; Γ |-- tCase indpar p c brs : tApp p (c :: args)
+    Σ ;;; Γ |-- tCase indpar p c brs : tApp p (List.skipn (snd indpar) args ++ [c])
 
 | type_Proj p c :
-    Σ ; Γ |-- tProj p c : tSort sSet (* FIXME *)
+    Σ ;;; Γ |-- tProj p c : tSort sSet (* FIXME *)
 
 | type_Fix mfix n :
     forall (isdecl : n < List.length mfix),
-    let ty := (safe_nth mfix (exist _ n isdecl)).(dtype _) in
+    let ty := (safe_nth mfix (exist _ n isdecl)).(dtype) in
     (** TODO check well-formed fix *)
-    Σ ; Γ |-- tFix mfix n : ty
+    Σ ;;; Γ |-- tFix mfix n : ty
 
 | type_CoFix mfix n :
     forall (isdecl : n < List.length mfix),
-    let ty := (safe_nth mfix (exist _ n isdecl)).(dtype _) in
+    let ty := (safe_nth mfix (exist _ n isdecl)).(dtype) in
     (** TODO check well-formed cofix *)
-    Σ ; Γ |-- tCoFix mfix n : ty
+    Σ ;;; Γ |-- tCoFix mfix n : ty
 
-| type_Conv t A B :
-    Σ ; Γ |-- t : A -> Σ ; Γ |-- A = B ->
-    Σ ; Γ |-- t : B          
+| type_Conv t A B s :
+    Σ ;;; Γ |-- t : A ->
+    Σ ;;; Γ |-- B : tSort s ->
+    Σ ;;; Γ |-- A <= B ->
+    Σ ;;; Γ |-- t : B          
 
-where " Σ ; Γ |-- t : T " := (@typing Σ Γ t T)
+where " Σ ;;; Γ |-- t : T " := (@typing Σ Γ t T) : type_scope
 
 with typing_spine (Σ : global_context) (Γ : context) : term -> list term -> term -> Prop :=
 | type_spine_nil ty : typing_spine Σ Γ ty [] ty
 | type_spine_const hd tl na A B B' :
-    Σ ; Γ |-- hd : A ->
+    Σ ;;; Γ |-- hd : A ->
     typing_spine Σ Γ (subst0 hd B) tl B' ->
     typing_spine Σ Γ (tProd na A B) (cons hd tl) B'
                      
-with conv (Σ : global_context) (Γ : context) : term -> term -> Prop :=
-| conv_refl t u : eq_term t u = true -> conv Σ Γ t u
-| conv_red_l t u v : red1 Σ Γ t v -> conv Σ Γ v u -> conv Σ Γ t u
-| conv_red_r t u v : conv Σ Γ t v -> red1 Σ Γ u v -> conv Σ Γ t u
+with cumul (Σ : global_context) (Γ : context) : term -> term -> Prop :=
+| cumul_refl t u : eq_term t u = true -> cumul Σ Γ t u
+| cumul_red_l t u v : red1 Σ Γ t v -> cumul Σ Γ v u -> cumul Σ Γ t u
+| cumul_red_r t u v : cumul Σ Γ t v -> red1 Σ Γ u v -> cumul Σ Γ t u
 
-where " Σ ; Γ |-- t = u " := (@conv Σ Γ t u).
+where " Σ ;;; Γ |-- t <= u " := (@cumul Σ Γ t u) : type_scope.
+
+Definition conv Σ Γ T U :=
+  Σ ;;; Γ |-- T <= U /\ Σ ;;; Γ |-- U <= T.
+
+Notation " Σ ;;; Γ |-- t = u " := (@conv Σ Γ t u) (at level 50, Γ, t, u at next level) : type_scope.
+
+
+Conjecture congr_cumul_prod : forall Σ Γ na na' M1 M2 N1 N2,
+    cumul Σ Γ M1 N1 ->
+    cumul Σ (Γ ,, vass na M1) M2 N2 ->
+    cumul Σ Γ (tProd na M1 M2) (tProd na' N1 N2).
 
 Fixpoint decompose_program (p : program) (env : global_context) : global_context * term :=
   match p with
@@ -613,7 +700,7 @@ Inductive type_constructors (Σ : global_context) (Γ : context) :
   list (ident * term * nat) -> Prop :=
 | type_cnstrs_nil : type_constructors Σ Γ []
 | type_cnstrs_cons id t s n l :
-    Σ ; Γ |-- t : tSort s ->
+    Σ ;;; Γ |-- t : tSort s ->
     type_constructors Σ Γ l ->
     (** TODO: check it has n products ending in a tRel application *)              
     type_constructors Σ Γ ((id, t, n) :: l).
@@ -622,7 +709,7 @@ Definition arities_context (l : list (ident * term * inductive_body)) :=
   List.map (fun '(na, t, _) => vass (nNamed na) t) l.
 
 Definition isType (Σ : global_context) (Γ : context) (t : term) :=
-  exists s, Σ ; Γ |-- t : tSort s.
+  exists s, Σ ;;; Γ |-- t : tSort s.
 
 Inductive type_inddecls (Σ : global_context) (Γ : context) :
   list (ident * term * inductive_body) -> Prop :=
@@ -639,15 +726,22 @@ Definition type_inductive Σ inds :=
   (** FIXME: should be pars ++ arities w/o params *)
   type_inddecls Σ (arities_context inds) inds.
                  
-Inductive type_global_env : global_context -> Set :=
+Inductive fresh_global (s : string) : global_context -> Prop :=
+| fresh_global_nil : fresh_global s nil
+| fresh_global_cons env g :
+    fresh_global s env -> global_decl_ident g <> s ->
+    fresh_global s (cons g env).
+  
+Inductive type_global_env : global_context -> Prop :=
 | globenv_nil : type_global_env []
 | globenv_cst Σ id ty trm :
     type_global_env Σ ->
-    Σ ; [] |-- trm : ty ->
+    fresh_global id Σ ->
+    Σ ;;; [] |-- trm : ty ->
     type_global_env (ConstantDecl id ty trm :: Σ)                     
 | globenv_ax Σ id ty s :
     type_global_env Σ ->
-    Σ ; [] |-- ty : tSort s ->
+    Σ ;;; [] |-- ty : tSort s ->
     type_global_env (AxiomDecl id ty :: Σ)
 | globenv_ind Σ ind m inds :
     type_global_env Σ ->
@@ -656,7 +750,7 @@ Inductive type_global_env : global_context -> Set :=
 
 Definition type_program (p : program) (ty : term) : Prop :=
   let '(Σ, t) := decompose_program p [] in
-  Σ ; [] |-- t : ty.
+  Σ ;;; [] |-- t : ty.
 
 Quote Recursively Definition foo := 0.
 
@@ -664,12 +758,12 @@ Require Import Omega.
 
 Ltac setenv na :=
   match goal with
-    |- ?Σ ; ?Γ |-- _ : _ => set(na := Σ)
+    |- ?Σ ;;; ?Γ |-- _ : _ => set(na := Σ)
   end.
 
 Ltac construct :=
   match goal with
-    |- ?Σ ; ?Γ |-- tConstruct ?c ?i : _ =>
+    |- ?Σ ;;; ?Γ |-- tConstruct ?c ?i : _ =>
     let H := fresh in let H' := fresh in
     unshelve assert(H:declared_constructor Σ (c,i)) by repeat econstructor;
     try (simpl; omega); assert(H':=type_Construct Σ Γ c i H); simpl in H';
@@ -707,69 +801,218 @@ Ltac fill_tApp :=
     |- context[mktApp _ ?x] => unify x (@nil term)
   end.
 
+Class Monad@{d c} (m : Type@{d} -> Type@{c}) : Type :=
+{ ret : forall {t : Type@{d}}, t -> m t
+; bind : forall {t u : Type@{d}}, m t -> (t -> m u) -> m u
+}.
+
+Class MonadExc E (m : Type -> Type) : Type :=
+{ raise : forall {T}, E -> m T
+; catch : forall {T}, m T -> (E -> m T) -> m T
+}.
+
+Module MonadNotation.
+
+  Delimit Scope monad_scope with monad.
+
+  Notation "c >>= f" := (@bind _ _ _ _ c f) (at level 50, left associativity) : monad_scope.
+  Notation "f =<< c" := (@bind _ _ _ _ c f) (at level 51, right associativity) : monad_scope.
+
+  Notation "x <- c1 ;; c2" := (@bind _ _ _ _ c1 (fun x => c2))
+    (at level 100, c1 at next level, right associativity) : monad_scope.
+
+  Notation "e1 ;; e2" := (_ <- e1%monad ;; e2%monad)%monad
+    (at level 100, right associativity) : monad_scope.
+
+End MonadNotation.
+Import MonadNotation.
+Instance option_monad : Monad option :=
+  {| ret A a := Some a ;
+     bind A B m f :=
+       match m with
+       | Some a => f a
+       | None => None
+       end
+  |}.
+
+Open Scope monad.
+
+Section MapOpt.
+  Context {A} (f : A -> option A).
+
+  Fixpoint mapopt (l : list A) : option (list A) :=
+    match l with
+    | nil => ret nil
+    | x :: xs => x' <- f x ;;
+                 xs' <- mapopt xs ;;
+                 ret (x' :: xs')
+    end.                                 
+End MapOpt.
+
+Module RedFlags.
+
+  Record t := mk
+    { beta : bool;
+      iota : bool;
+      zeta : bool;
+      delta : bool;
+      fix_ : bool;
+      cofix_ : bool }.
+
+  Definition default := mk true true true true true true.
+End RedFlags.
+
 Section Reduce.
+  Context (flags : RedFlags.t).
+
   Context (Σ : global_context).
+
+  Definition zip (t : term * list term) := tAppnil (fst t) (snd t).
   
-  Fixpoint reduce (n : nat) (t : term) : term :=
-  match n with 0 => t | S n =>
+  Fixpoint reduce_stack (Γ : context) (n : nat) (t : term) (stack : list term)
+    : option (term * list term) :=      
+  match n with 0 => None | S n =>
   match t with
-  | tApp (tLambda _ _ b) (a :: l) => reduce n (subst0 a b)
-  | tCase _ _ (tConstruct ind c) brs => reduce n (iota_red c [] brs)
-  | tCase _ _ (tApp (tConstruct ind c) args) brs => reduce n (iota_red c args brs)
+
+  | tRel c =>
+    if RedFlags.zeta flags then
+      d <- nth_error Γ c ;;
+      match d.(decl_body) with
+      | None => ret (t, stack)
+      | Some b => reduce_stack Γ n (lift0 (S c) b) stack
+      end
+    else ret (t, stack)
+    
+  | tLetIn _ b _ c =>
+    if RedFlags.zeta flags then
+      reduce_stack Γ n (subst0 b c) stack
+    else ret (t, stack)
+
   | tConst c =>
-    match lookup_env Σ c with
-    | Some (ConstantDecl _ _ body) => reduce n body
-    | _ => t
-    end
-  (* | tRel c => *)
-  (*   match nth_error Γ c with *)
-  (*   | Some d => match d.(decl_body) with None => t | Some b => reduce n b end *)
-  (*   | None => t *)
-  (*   end *)
-  | tApp f args =>
-    reduce n (tApp (reduce n f) (List.map (reduce n) args))
-  | tProd na b t => tProd na (reduce n b) (reduce n t)
-  | _ => t
+    if RedFlags.delta flags then
+      match lookup_env Σ c with
+      | Some (ConstantDecl _ _ body) => reduce_stack Γ n body stack
+      | _ => ret (t, stack)
+      end
+    else ret (t, stack)
+
+  | tApp f args => reduce_stack Γ n f (args ++ stack)
+
+  | tLambda na ty b =>
+    if RedFlags.beta flags then
+      match stack with
+      | a :: args' =>
+        (** CBV reduction: we reduce arguments before substitution *)
+        a' <- reduce_stack Γ n a [] ;;
+        reduce_stack Γ n (subst0 (zip a') b) args'
+      | _ => b' <- reduce_stack (Γ ,, vass na ty) n b stack ;;
+               ret (tLambda na ty (zip b'), stack)
+      end
+    else ret (t, stack)
+      
+  | tFix mfix idx =>
+    if RedFlags.fix_ flags then
+      nf <- unfold_fix mfix idx ;;
+      let '(narg, fn) := nf in
+      match  List.nth_error stack narg with
+      | Some c =>
+        c' <- reduce_stack Γ n c [] ;;
+        match fst c' with
+        | tConstruct _ _ => reduce_stack Γ n fn stack
+        | _ => ret (t, stack)
+        end
+      | _ => ret (t, stack)
+      end
+    else ret (t, stack)
+
+  | tProd na b t =>
+    b' <- reduce_stack Γ n b [] ;;
+    t' <- reduce_stack (Γ ,, vass na (zip b')) n t [] ;;
+    ret (tProd na (zip b') (zip t'), stack)
+
+  | tCast c _ _ => reduce_stack Γ n c stack
+
+  | tCase (ind, par) p c brs =>
+    if RedFlags.iota flags then
+      c' <- reduce_stack Γ n c [] ;;
+      match c' with
+      | (tConstruct ind c, args) => reduce_stack Γ n (iota_red par c args brs) stack
+      | _ => ret (tCase (ind, par) p (zip c') brs, stack)
+      end
+    else ret (t, stack)
+
+  | _ => ret (t, stack)
+
   end
   end.
+
+  Definition reduce_stack_term Γ n c :=
+    res <- reduce_stack Γ n c [] ;;
+    ret (zip res).
+  
+  Definition fix_decls (l : mfixpoint term) :=
+    let fix aux acc ds :=
+        match ds with
+        | nil => acc
+        | d :: ds => aux (vass d.(dname) d.(dtype) :: acc) ds
+        end
+    in aux [] l.
+
+  Definition map_constr_with_binders (f : context -> term -> term) Γ (t : term) : term :=
+    match t with
+    | tRel i => t
+    | tEvar ev args => tEvar ev (List.map (f Γ) args)
+    | tLambda na T M => tLambda na (f Γ T) (f Γ M)
+    | tApp u v => tApp (f Γ u) (List.map (f Γ) v)
+    | tProd na A B =>
+      let A' := f Γ A in
+      tProd na A' (f (Γ ,, vass na A') B)
+    | tCast c kind t => tCast (f Γ c) kind (f Γ t)
+    | tLetIn na b t b' =>
+      let b' := f Γ b in
+      let t' := f Γ t in
+      tLetIn na b' t' (f (Γ ,, vdef na b' t') b')
+    | tCase ind p c brs =>
+      let brs' := List.map (on_snd (f Γ)) brs in
+      tCase ind (f Γ p) (f Γ c) brs'
+    | tProj p c => tProj p (f Γ c)
+    | tFix mfix idx =>
+      let Γ' := fix_decls mfix ++ Γ in
+      let mfix' := List.map (map_def (f Γ')) mfix in
+      tFix mfix' idx
+    | tCoFix mfix k =>
+      let Γ' := fix_decls mfix ++ Γ in
+      let mfix' := List.map (map_def (f Γ')) mfix in
+      tCoFix mfix' k
+    | x => x
+    end.
+  
+  Fixpoint reduce_opt Γ n c :=
+    match n with
+    | 0 => None
+    | S n =>
+      match reduce_stack_term Γ n c with
+      | Some c' =>
+        Some (map_constr_with_binders
+                (fun Γ t => match reduce_opt Γ n t with Some t => t | None => t end) Γ c')
+      | None => None
+      end
+    end.
+
 End Reduce.
 
-Axiom reduce_sym : forall Σ Γ t u, Σ ; Γ |-- t = u -> Σ ; Γ |-- u = t.
-Axiom reduce_trans : forall Σ Γ t u v, Σ ; Γ |-- t = u -> Σ ; Γ |-- u = v -> Σ ; Γ |-- t = v.
+Axiom conv_refl : forall Σ Γ t, Σ ;;; Γ |-- t = t.
+Axiom cumul_refl' : forall Σ Γ t, Σ ;;; Γ |-- t <= t.
+Axiom cumul_trans : forall Σ Γ t u v, Σ ;;; Γ |-- t <= u -> Σ ;;; Γ |-- u <= v -> Σ ;;; Γ |-- t <= v.
 
-Conjecture reduce_conv : forall Σ Γ n t, Σ ; Γ |-- reduce Σ n t = t.
-
-Lemma reduce_conv_prf n : forall Σ Γ t u,
-    Σ ; Γ |-- reduce Σ n t = reduce Σ n u ->
-    Σ ; Γ |-- t = u.
-Proof.
-  intros. eapply reduce_trans. eapply reduce_sym.
-  apply reduce_conv with (n:=n).
-  eapply reduce_trans. eapply H. eapply reduce_conv.
-Qed.
-
-Ltac reduce :=
-  apply (reduce_conv_prf 100); simpl; try solve [ repeat constructor ].
-
-Hint Extern 10 => fill_tApp : typecheck.
-Hint Extern 5 => construct : typecheck.
-Hint Extern 100 => progress simpl : typecheck.
-Hint Extern 100 => econstructor : typecheck.
-
-
-Quote Recursively Definition matc :=
-  match 0 with
-  | 0 => 0
-  | S x => x
+Hint Resolve conv_refl cumul_refl' : typecheck.
+Definition try_reduce Σ Γ n t :=
+  match reduce_opt RedFlags.default Σ Γ n t with
+  | Some t' => t'
+  | None => t
   end.
 
-Example mat : type_program matc natr.
-Proof.
-  start.
-  eapply type_Conv.
-  eauto with typecheck.
-  reduce.
-Qed.
+Conjecture reduce_cumul : forall Σ Γ n t, Σ ;;; Γ |-- try_reduce Σ Γ n t <= t.
 
 Quote Recursively Definition matc' :=
   (fun y => match y with
@@ -779,15 +1022,669 @@ Quote Recursively Definition matc' :=
 
 Definition timpl x y := tProd nAnon x (lift0 1 y).
 
-Example mat' : type_program matc' (timpl natr natr).
+Class Fuel := { fuel : nat }.
+
+Section Typecheck.
+  Context `{F:Fuel}.
+  Context (Σ : global_context).
+  
+  Inductive type_error :=
+  | UnboundRel (n : nat)
+  | UnboundVar (id : string)
+  | UnboundMeta (m : nat)
+  | UnboundEvar (ev : nat)
+  | UndeclaredConstant (c : string)
+  | UndeclaredInductive (c : inductive)
+  | UndeclaredConstructor (c : inductive) (i : nat)
+  | NotConvertible (Γ : context) (t u t' u' : term)
+  | NotASort (t : term)
+  | NotAProduct (t t' : term)
+  | NotAnInductive (t : term)
+  | IllFormedFix (m : mfixpoint term) (i : nat)
+  | NotEnoughFuel (n : nat).
+  
+  Inductive typing_result (A : Type) :=
+  | OfType (a : A)
+  | TypeError (t : type_error).
+  Global Arguments OfType {A} a.
+  Global Arguments TypeError {A} t.
+  
+  Instance typing_monad : Monad typing_result :=
+    {| ret A a := OfType a ;
+       bind A B m f :=
+        match m with
+        | OfType a => f a
+        | TypeError t => TypeError t
+        end
+    |}.
+
+  Instance monad_exc : MonadExc type_error typing_result :=
+    { raise A e := TypeError e;
+      catch A m f :=
+        match m with
+        | OfType a => m
+        | TypeError t => f t
+        end
+    }.
+
+  Definition hnf_stack Σ Γ t :=
+    match reduce_stack RedFlags.default Σ Γ fuel t [] with
+    | Some t' => ret t'
+    | None => raise (NotEnoughFuel fuel)
+    end.
+
+  Definition reduce Σ Γ t :=
+    match reduce_opt RedFlags.default Σ Γ fuel t with
+    | Some t' => ret t'
+    | None => raise (NotEnoughFuel fuel)
+    end.
+  
+  Definition convert_leq Γ (t u : term) : typing_result unit :=
+    if eq_term t u then ret ()
+    else 
+      t' <- reduce Σ Γ t ;;
+      u' <- reduce Σ Γ u ;;
+      if leq_term t' u' then ret ()
+      else raise (NotConvertible Γ t u t' u').
+
+  Definition reduce_to_sort Γ (t : term) : typing_result sort :=
+    t' <- hnf_stack Σ Γ t ;;
+    match t' with
+    | (tSort s, []) => ret s
+    | _ => raise (NotASort t)
+    end.
+
+  Definition reduce_to_prod Γ (t : term) : typing_result (term * term) :=
+    t' <- hnf_stack Σ Γ t ;;
+    match t' with
+    | (tProd _ a b,[]) => ret (a, b)
+    | _ => raise (NotAProduct t (zip t'))
+    end.
+
+  Definition reduce_to_ind Γ (t : term) : typing_result (inductive * list term) :=
+    t' <- hnf_stack Σ Γ t ;;
+    match t' with
+    | (tInd i, l) => ret (i, l)
+    | _ => raise (NotAnInductive t)
+    end.
+
+  Section InferAux.
+    Variable (infer : context -> term -> typing_result term).
+
+    Fixpoint infer_spine
+             (Γ : context) (ty : term) (l : list term) {struct l} : typing_result term :=
+    match l with
+    | nil => ret ty
+    | cons x xs =>
+       pi <- reduce_to_prod Γ ty ;;
+       let '(a1, b1) := pi in
+       tx <- infer Γ x ;;
+       convert_leq Γ tx a1 ;;
+       infer_spine Γ (subst0 x b1) xs
+    end.
+
+    Definition infer_type Γ t :=
+      tx <- infer Γ t ;;
+      reduce_to_sort Γ tx.
+
+    Definition infer_cumul Γ t t' :=
+      tx <- infer Γ t ;;
+      convert_leq Γ tx t'.
+    
+  End InferAux.
+
+  Definition lookup_constant_type cst :=
+    match lookup_env Σ cst with
+      | Some (ConstantDecl _ ty _) => ret ty
+      | Some (AxiomDecl _ ty) => ret ty
+      |  _ => raise (UndeclaredConstant cst)
+    end.
+  
+  Fixpoint infer (Γ : context) (t : term) : typing_result term :=
+    match t with
+    | tRel n =>
+      match nth_error Γ n with
+      | Some d => ret (lift0 (S n) d.(decl_type))
+      | None => raise (UnboundRel n)
+      end
+
+    | tVar n => raise (UnboundVar n)
+    | tMeta n => raise (UnboundMeta n)
+    | tEvar ev args => raise (UnboundEvar ev)
+      
+    | tSort s => ret (tSort (succ_sort s))
+
+    | tCast c k t =>
+      infer_type infer Γ t ;;
+      infer_cumul infer Γ c t ;;
+      ret t
+
+    | tProd n t b =>
+      s1 <- infer_type infer Γ t ;;
+      s2 <- infer_type infer (Γ ,, vass n t) b ;;
+      ret (tSort (max_sort s1 s2))
+
+    | tLambda n t b =>
+      infer_type infer Γ t ;;
+      t2 <- infer (Γ ,, vass n t) b ;;
+      ret (tProd n t t2)
+
+    | tLetIn n b b_ty b' =>
+      infer_type infer Γ b_ty ;;
+       infer_cumul infer Γ b b_ty ;;
+       b'_ty <- infer (Γ ,, vdef n b b_ty) b' ;;
+       ret (tLetIn n b b_ty b'_ty)
+
+    | tApp t l =>
+      t_ty <- infer Γ t ;;
+      infer_spine infer Γ t_ty l
+       
+    | tConst cst => lookup_constant_type cst
+
+    | tInd (mkInd ind i) =>
+      match lookup_env Σ ind with
+      | Some (InductiveDecl _ _ l) =>
+        match nth_error l i with
+        | Some (_, ty, _) => ret ty
+        | None => raise (UndeclaredInductive (mkInd ind i))
+        end
+      |  _ => raise (UndeclaredInductive (mkInd ind i))
+      end
+
+    | tConstruct (mkInd ind i) k =>
+      match lookup_env Σ ind with
+      | Some (InductiveDecl _ _ l) =>
+        match nth_error l i with
+        | Some (_, _, mkinductive_body cstrs) =>
+          match nth_error cstrs k with
+          | Some (_, ty, _) =>
+            ret (substl (inds ind l) ty)
+          | None => raise (UndeclaredConstructor (mkInd ind i) k)
+          end
+        | None => raise (UndeclaredInductive (mkInd ind i))
+        end
+      |  _ => raise (UndeclaredInductive (mkInd ind i))
+      end
+        
+    | tCase (ind, par) p c brs =>
+      ty <- infer Γ c ;;
+      indargs <- reduce_to_ind Γ ty ;;
+      (** TODO check branches *)
+      let '(ind', args) := indargs in
+      if eq_ind ind ind' then
+        ret (tApp p (List.skipn par args ++ [c]))
+      else
+        let ind1 := tInd ind in
+        let ind2 := tInd ind' in
+        raise (NotConvertible Γ ind1 ind2 ind1 ind2)
+
+    | tProj p c =>
+      ty <- infer Γ c ;;
+      indargs <- reduce_to_ind Γ ty ;;
+      (* FIXME *)
+      ret ty 
+      
+    | tFix mfix n =>
+      match nth_error mfix n with
+      | Some f => ret f.(dtype)
+      | None => raise (IllFormedFix mfix n)
+      end
+
+    | tCoFix mfix n =>
+      match nth_error mfix n with
+      | Some f => ret f.(dtype)
+      | None => raise (IllFormedFix mfix n)
+      end
+    end.
+
+  Definition check (Γ : context) (t : term) (ty : term) : typing_result unit :=
+    infer Γ ty ;;
+    infer_cumul infer Γ t ty ;;
+    ret ().
+
+  Definition typechecking (Γ : context) (t ty : term) :=
+    match check Γ t ty with
+    | OfType _ => true
+    | TypeError _ => false
+    end.
+
+    
+    Lemma nth_error_safe_nth {A} n (l : list A) (isdecl : n < Datatypes.length l) :
+      nth_error l n = Some (safe_nth l (exist _ n isdecl)).
+    Proof.
+      revert n isdecl; induction l; intros.
+      - inversion isdecl.
+      - destruct n as [| n']; simpl.
+        reflexivity.
+        simpl in IHl.
+        simpl in isdecl.
+        now rewrite <- IHl.
+    Qed.
+
+  Ltac tc := eauto with typecheck.
+
+  Arguments bind _ _ _ _ ! _.
+  Open Scope monad.
+
+  Conjecture cumul_convert_leq : forall Γ t t',
+    Σ ;;; Γ |-- t <= t' <-> convert_leq Γ t t' = OfType ().
+
+  Conjecture cumul_reduce_to_sort : forall Γ t s',
+      Σ ;;; Γ |-- t <= tSort s' <->
+      exists s'', reduce_to_sort Γ t = OfType s'' /\ leq_sort s'' s' = true.
+
+  Conjecture cumul_reduce_to_product : forall Γ t na a b,
+      Σ ;;; Γ |-- t <= tProd na a b ->
+      exists a' b',
+        reduce_to_prod Γ t = OfType (a', b') /\
+        cumul Σ Γ (tProd na a' b') (tProd na a b).
+
+  Conjecture cumul_reduce_to_ind : forall Γ t i args,
+      Σ ;;; Γ |-- t <= mktApp (tInd i) args <->
+      exists args',
+        reduce_to_ind Γ t = OfType (i, args') /\
+        cumul Σ Γ (mktApp (tInd i) args') (mktApp (tInd i) args).
+
+  Lemma lookup_constant_type_declared cst (isdecl : declared_constant Σ cst) :
+    lookup_constant_type cst = OfType (type_of_constant Σ (exist _ _ isdecl)).
+  Proof.
+    unfold lookup_constant_type.
+    destruct isdecl as [d [H H']].
+    rewrite H at 1.
+    
+    induction Σ. simpl. bang. simpl. destruct dec. simpl.
+    unfold type_of_constant_decl. simpl.
+    simpl in H. pose proof H. rewrite e in H0.
+    injection H0 as ->.
+    destruct d; auto. bang.
+
+    simpl in H. pose proof H. rewrite e in H0.
+    specialize (IHg H0).
+    rewrite IHg at 1. f_equal. pi.
+  Qed.
+
+  Lemma lookup_constant_type_is_declared cst T :
+    lookup_constant_type cst = OfType T -> declared_constant Σ cst.
+  Proof.
+    unfold lookup_constant_type, declared_constant.
+    destruct lookup_env; try discriminate.
+    destruct g; intros; try discriminate.
+    eexists. split; eauto.
+    eexists. split; eauto.
+  Qed.
+  
+  Lemma eq_ind_refl i i' : eq_ind i i' = true <-> i = i'.
+  Admitted.
+
+  Lemma infer_complete Γ t T :
+    Σ ;;; Γ |-- t : T -> exists T', infer Γ t = OfType T' /\ cumul Σ Γ T' T.
+  Proof.
+    induction 1; unfold infer_type, infer_cumul in *; simpl; unfold infer_type, infer_cumul in *;
+      repeat match goal with
+        H : exists T', _ |- _ => destruct H as [? [-> H]]
+      end; simpl; try (eexists; split; [ reflexivity | solve [ tc ] ]).
+
+    - eexists. rewrite (nth_error_safe_nth n _ isdecl).
+      split; [ reflexivity | tc ]. 
+
+    - eexists.
+      apply cumul_reduce_to_sort in IHtyping1 as [s'' [-> Hs'']].
+      apply cumul_convert_leq in IHtyping2 as ->.
+      simpl. split; tc.
+
+    - apply cumul_reduce_to_sort in IHtyping1 as [s'' [-> Hs'']].
+      apply cumul_reduce_to_sort in IHtyping2 as [s''' [-> Hs''']].
+      simpl. eexists; split; tc.
+      admit.
+      
+    - eexists. apply cumul_reduce_to_sort in IHtyping1 as [s'' [-> Hs'']].
+      split. reflexivity.
+      apply congr_cumul_prod; tc.
+
+    - apply cumul_convert_leq in IHtyping2 as ->; simpl.
+      eexists ; split; tc.
+      admit.
+      
+    - admit.
+
+    - erewrite lookup_constant_type_declared.
+      eexists ; split; [ reflexivity | tc ].
+
+    - admit.
+    - admit.
+
+    - destruct indpar.
+      apply cumul_reduce_to_ind in IHtyping as [args' [-> Hcumul]].
+      simpl in *. rewrite (proj2 (eq_ind_refl i i) eq_refl). 
+      eexists ; split; [ reflexivity | tc ].
+      admit.
+
+    - admit.
+
+    - eexists.
+      rewrite (nth_error_safe_nth _ _ isdecl).
+      split; [ reflexivity | tc ].
+
+    - eexists.
+      rewrite (nth_error_safe_nth _ _ isdecl).
+      split; [ reflexivity | tc ].
+
+    - eexists.
+      split; [ reflexivity | tc ].
+      eapply cumul_trans; eauto.
+
+  Admitted.
+  Lemma nth_error_isdecl {A} {l : list A} {n c} : nth_error l n = Some c -> n < Datatypes.length l.
+  Proof.
+    intros.
+    rewrite <- nth_error_Some. intro H'. rewrite H' in H; discriminate.
+  Qed.
+      
+  Ltac infers :=
+    repeat
+      match goal with
+      | |- context [infer ?Γ ?t] =>
+        destruct (infer Γ t) eqn:?; [ simpl | simpl; intro; discriminate ]
+      | |- context [infer_type ?Γ ?t] =>
+        destruct (infer_type Γ t) eqn:?; [ simpl | simpl; intro; discriminate ]
+      | |- context [infer_cumul ?Γ ?t ?t2] =>
+        destruct (infer_cumul Γ t t2) eqn:?; [ simpl | simpl; intro; discriminate ]
+      | |- context [convert_leq ?Γ ?t ?t2] =>
+        destruct (convert_leq Γ t t2) eqn:?; [ simpl | simpl; intro; discriminate ]
+      end; try intros [= <-].
+
+  Lemma leq_sort_refl x : leq_sort x x = true.
+  Proof. destruct x; reflexivity. Qed.
+  Hint Resolve leq_sort_refl : typecheck.
+  Lemma infer_type_correct Γ t x :
+    (forall (Γ : context) (T : term), infer Γ t = OfType T -> Σ;;; Γ |-- t : T) ->
+    infer_type infer Γ t = OfType x ->
+    Σ ;;; Γ |-- t : tSort x.                            
+  Proof.
+    intros IH H.
+    unfold infer_type in H.
+    revert H; infers.
+    specialize (IH _ _ Heqt0).
+    intros.
+    eapply type_Conv. apply IH.
+    constructor.
+    rewrite cumul_reduce_to_sort. exists x. split; tc.
+  Qed.
+
+  Lemma infer_cumul_correct Γ t u x x' :
+    (forall (Γ : context) (T : term), infer Γ u = OfType T -> Σ;;; Γ |-- u : T) ->
+    (forall (Γ : context) (T : term), infer Γ t = OfType T -> Σ;;; Γ |-- t : T) ->
+    infer_type infer Γ u = OfType x' ->
+    infer_cumul infer Γ t u = OfType x ->
+    Σ ;;; Γ |-- t : u.                            
+  Proof.
+    intros IH IH' H H'.
+    unfold infer_cumul in H'.
+    revert H'; infers. 
+    specialize (IH' _ _ Heqt0).
+    intros.
+    eapply type_Conv. apply IH'.
+    apply infer_type_correct; eauto.
+    destruct a0. now rewrite cumul_convert_leq.
+  Qed.
+
+  Lemma nth_error_Some_safe_nth A (l : list A) n c :
+    nth_error l n = Some c -> exists isdecl,
+      safe_nth l (exist _ n isdecl) = c.
+  Proof.
+    intros H.
+    pose proof H.
+    pose proof (nth_error_safe_nth _ _ (nth_error_isdecl H0)).
+    rewrite H in H1.
+    eexists. injection H1 as <-. reflexivity.
+  Qed.
+
+  
+  Ltac infco := eauto using infer_cumul_correct, infer_type_correct.
+  Lemma infer_correct Γ t T :
+    infer Γ t = OfType T -> Σ ;;; Γ |-- t : T.
+  Proof.
+    induction t in Γ, T |- * ; simpl; intros; try discriminate;
+      revert H; infers; try solve [econstructor; infco].
+    
+    - destruct nth_error eqn:Heq; try discriminate.
+      destruct (nth_error_Some_safe_nth _ _ _ _ Heq) as [isdecl <-].
+      intros [= <-]. constructor.
+
+    - admit.
+
+    - intros.
+      pose proof (lookup_constant_type_declared _ (lookup_constant_type_is_declared _ _ H)).
+      rewrite H in H0 at 1.
+      injection H0 as ->. tc.
+      constructor.
+      
+    - (* Ind *) admit.
+
+    - (* Construct *) admit.
+
+    - (* Case *)
+      destruct p.
+      infers.
+      destruct reduce_to_ind eqn:?; try discriminate. simpl.
+      destruct a0 as [ind' args].
+      destruct eq_ind eqn:?; try discriminate.
+      intros [= <-].
+      eapply type_Case. simpl in *.
+      eapply type_Conv. eauto.
+      admit.
+      rewrite cumul_reduce_to_ind.
+      exists args. split; auto.
+      rewrite Heqt0. repeat f_equal. apply eq_ind_refl in Heqb. congruence.
+      tc.
+
+    - (* Proj *) admit.
+
+    - destruct nth_error eqn:?; intros [= <-].
+      destruct (nth_error_Some_safe_nth _ _ _ _ Heqo) as [isdecl <-].
+      constructor.
+
+    - destruct nth_error eqn:?; intros [= <-].
+      destruct (nth_error_Some_safe_nth _ _ _ _ Heqo) as [isdecl <-].
+      constructor.
+  Admitted.
+
+End Typecheck.
+
+Quote Recursively Definition four := (2 + 2).
+
+Ltac typecheck := start;
+  match goal with
+    |- ?Σ ;;; ?Γ |-- ?t : ?T =>
+    eapply (infer_correct Σ Γ t T); vm_compute; reflexivity
+  end.
+Ltac infer := start;
+  match goal with
+    |- ?Σ ;;; ?Γ |-- ?t : ?T => 
+    eapply (infer_correct Σ Γ t T);
+      let t' := eval vm_compute in (infer Σ Γ t) in
+          change (t' = OfType T); reflexivity
+  end.
+
+Instance default_fuel : Fuel := { fuel := 2 ^ 18 }.
+
+Example typecheck_four : type_program four natr := ltac:(typecheck).
+
+Goal exists ty, type_program four ty.
 Proof.
-  start.
-  eapply type_Conv.
-  eauto with typecheck.
-  econstructor.
-  econstructor.
-  eauto with typecheck.
-  reduce.
-  Unshelve.
-  simpl. omega.
+  eexists. infer.
 Qed.
+
+Fixpoint fresh id env : bool :=
+  match env with
+  | nil => true
+  | cons g env => negb (eq_constant (global_decl_ident g) id) && fresh id env
+  end.
+
+Section Checker.
+
+  Context `{F:Fuel}.
+
+  Inductive env_error :=
+  | IllFormedDecl (e : string) (e : type_error)
+  | AlreadyDeclared (id : string).
+
+  Inductive EnvCheck (A : Type) :=
+  | CorrectDecl (a : A)
+  | EnvError (e : env_error).
+  Global Arguments EnvError {A} e.
+  Global Arguments CorrectDecl {A} a.
+  
+  Instance envcheck_monad : Monad EnvCheck :=
+    {| ret A a := CorrectDecl a ;
+       bind A B m f :=
+         match m with
+         | CorrectDecl a => f a
+         | EnvError e => EnvError e
+         end
+    |}.
+
+  Definition wrap_error {A} (id : string) (check : typing_result A) : EnvCheck A :=
+    match check with
+    | OfType a => CorrectDecl a
+    | TypeError e => EnvError (IllFormedDecl id e)
+    end.
+
+  Definition check_wf_type id Σ t :=
+    wrap_error id (infer_type Σ (infer Σ) [] t) ;; ret ().
+
+  Definition check_wf_judgement id Σ t ty :=
+    wrap_error id (check Σ [] t ty) ;; ret ().
+
+  Definition infer_term Σ t :=
+    wrap_error "" (infer Σ [] t).
+  
+  Definition check_wf_decl Σ (g : global_decl) : EnvCheck () :=
+    match g with
+    | ConstantDecl id ty term =>
+      check_wf_judgement id Σ term ty
+    | AxiomDecl id ty => check_wf_type id Σ ty
+    | InductiveDecl id par inds =>
+      List.fold_left (fun acc '(id, ty, body) =>
+                        acc ;;
+                            check_wf_type id Σ ty) inds (ret ())
+                     
+    end.
+
+  Fixpoint check_fresh id env : EnvCheck () :=
+    match env with
+    | [] => ret ()
+    | g :: env =>
+      check_fresh id env;;
+      if eq_constant id (global_decl_ident g) then
+        EnvError (AlreadyDeclared id)
+      else ret ()
+    end.
+
+  Fixpoint check_wf_env (g : global_context) :=
+    match g with
+    | [] => ret ()
+    | g :: env =>
+      check_wf_env env ;;
+      check_wf_decl env g ;;
+      check_fresh (global_decl_ident g) env
+    end.
+
+  Definition typecheck_program (p : program) : EnvCheck term :=
+    let '(Σ, t) := decompose_program p [] in
+    check_wf_env Σ ;; infer_term Σ t.
+
+End Checker.
+
+Require Import Morphisms.
+Quote Recursively Definition idq := @Coq.Classes.Morphisms.Proper.
+
+Eval vm_compute in typecheck_program idq.
+
+Require Import Recdef.
+Require Import Coq.omega.Omega.
+Set Implicit Arguments.
+
+(** A function defined using measure or well-founded relation **)
+Function Plus1 (n: nat) {measure id n} : nat :=
+  match n with
+    | 0 => 1
+    | S p => S (Plus1 p)
+  end.
+- intros. unfold id. abstract omega.
+Defined.
+
+Require Import Coq.Lists.List.
+Require Import Coq.Strings.String.
+Require Import Coq.Strings.Ascii.
+Require Import Coq.Bool.Bool.
+Require Import Template.Template.
+Require Import Template.Ast.
+
+Unset Template Cast Propositions.
+
+(* Uase template-coq to make a [program] from function defined above *)
+(* Quote Recursively Definition p_Plus1 := Plus1. *)
+
+(* Eval native_compute in typecheck_program p_Plus1. *)
+
+Definition test_reduction (p : program) :=
+    let '(Σ, t) := decompose_program p [] in
+    reduce Σ [] t.
+
+Definition out_typing c :=
+  match c with
+  | OfType t => t
+  | TypeError e => tRel 0
+  end.
+
+Definition out_check c :=
+  match c with
+  | CorrectDecl t => t
+  | EnvError e => tRel 0
+  end.
+
+Ltac interp_red c :=
+  let t:= eval vm_compute in (out_typing (test_reduction c)) in exact t.
+
+Ltac interp_infer c :=
+  let t:= eval vm_compute in (out_check (typecheck_program c)) in exact t.
+
+Ltac term_type c :=
+  let X := type of c in exact X.
+
+Ltac quote_type c :=
+  let X := type of c in
+  quote_term X ltac:(fun Xast => exact Xast).
+
+Notation convertible x y := (@eq_refl _ x : x = y).
+
+Module Test1.
+  Definition term := (Nat.mul 2 62).
+  Load "test_term.v".
+End Test1.
+
+Module Test2.
+  Definition term := (fun (f : nat -> nat) (x : nat) => f (f x)).
+  Load "test_term.v".
+End Test2.
+
+Module Test3.
+  Definition term := (id 0).
+  Load "test_term.v".
+End Test3.
+
+Module Test4.
+  Definition term := @id.
+  Set Printing Universes.
+  Load "test_term.v".
+End Test4.
+
+(* Require Import ExtrOcamlBasic. *)
+(* Require Import ExtrOcamlString. *)
+
+(* Set Extraction Optimize. *)
+
+(* Recursive Extraction typecheck_program. *)
+(** Compile template_program using certicoq and bind to template, voilà: 
+    a certified typechecker of Coq vos! *)
